before splitting more files

concurrency/Modular/giveup_traverse.v
@@ -16,9 +16,11 @@ Definition t_struct_pn := Tstruct _pn noattr.
 
 Context {N: NodeRep}.
 
+About NodeRep.
+
 Definition node_rep  pn g g_current (r : node_info) :=
-    !!(repable_signed (number2Z r.1.2.1) ∧ repable_signed (number2Z r.1.2.2) /\
-         is_pointer_or_null r.1.1.2) &&
+    !!(repable_signed (number2Z r.1.2.1) ∧ repable_signed (number2Z r.1.2.2)
+       /\ is_pointer_or_null r.1.1.1 /\ is_pointer_or_null r.1.1.2 ) &&
       field_at Ews (t_struct_node) [StructField _t] r.1.1.1 pn *
       field_at Ews (t_struct_node) [StructField _min] (vint (number2Z (r.1.2.1))) pn * (*min*)
       field_at Ews (t_struct_node) [StructField _max] (vint (number2Z (r.1.2.2))) pn * (*max*)
@@ -97,15 +99,6 @@ Definition extract_lst_pn (m: mpredList) : list val :=
   | _ => []
   end.
 
-Lemma mylemm (a b : val): (Val.eq a b) -> a = b.
-Proof.
-  Compute (a <> b) /\ True.
-  Search and Prop.
-  intros.
-  destruct (Val.eq a b).
-  - admit.
-Admitted.
-  
 Definition pn_unique (pn : val) (lst : list mpredList) : Prop :=
   fold_right (fun r acc => ( pn <> pnL r) /\ acc) true lst.
 
@@ -234,8 +227,7 @@ Proof.
   - inversion H.
   - simpl in H0.
     inversion H; destruct H0.
-    + rewrite H1 in H0.
-      contradiction.
+    + by rewrite H1 in H0. 
     + specialize ((IHI H1) H2).
       apply IHI.
 Qed.
@@ -642,16 +634,35 @@ Program Definition traverse_spec :=
   PRE [ tptr t_struct_pn, tint]
   PROP (and (Z.le (Int.min_signed) x) (Z.le x (Int.max_signed)); is_pointer_or_null v)
   PARAMS (b; Vint (Int.repr x)) GLOBALS (gv)
-  SEP  (mem_mgr gv;
+  SEP  (mem_mgr gv; 
         in_tree g g_root n lock;
         !!(is_pointer_or_null lock /\ is_pointer_or_null n) && seplog.emp;
         EX (p: val), data_at Ews (t_struct_pn) (p, n) b ) | (CSS g g_root M)
   POST [ tint ]
-  EX  pt: enum * (val * (share * gname )) %type,
-  PROP () (* pt: enum * (val * (share * (gname * node_info))) *)
+  EX  pt: enum * (val * (share * (gname * node_info ))) %type,
+  PROP ()
   LOCAL (temp ret_temp (enums pt.1))
-  SEP (mem_mgr gv)| (CSS g g_root M).
+  SEP (mem_mgr gv; !!( key_in_range x (((pt.2.2.2).2).1).2 = true ∧
+                         repable_signed (number2Z (((pt.2.2.2).2).1).2.1) ∧
+                         repable_signed (number2Z (((pt.2.2.2).2).1).2.2) /\
+                         is_pointer_or_null ((((pt.2.2.2).2).1).1).2
+                       /\ (if Val.eq (enums pt.1) (enums NN) then
+                            pt.2.2.2.2.2 = Some None /\ ((((pt.2.2.2).2).1).1).1 = nullval
+                          else ((((pt.2.2.2).2).1).1).1 <> nullval)
+                        (* (match (pt.1 : enum) with
+                         | NN => pt.2.2.2.2.2 = Some None /\ ((((pt.2.2.2).2).1).1).1 = nullval
+                         | NF | F =>  ((((pt.2.2.2).2).1).1).1 <> nullval
+                        (* | NF => ((((pt.2.2.2).2).1).1).1 <> nullval *)
+                          end) *)  ) && seplog.emp; 
+        data_at Ews t_struct_pn (pt.2.1, pt.2.1) b;
+        in_tree g pt.2.2.2.1 pt.2.1 ((((pt.2.2.2).2).1).1).2;
+       node_lock_inv_pred g pt.2.1 pt.2.2.2.1 (pt.2.2.2).2
 
+
+
+  )| (CSS g g_root M).
+
+Check enums _.
 (* t_struct_node represents for the generic-struct rather specific-data-structure *)
 (* Spec of inrange function *)
 Definition inRange_spec :=
@@ -674,6 +685,22 @@ Definition inRange_spec :=
              field_at sh (t_struct_node) [StructField _min] (Vint (Int.repr min)) p;
               field_at sh (t_struct_node) [StructField _max] (Vint (Int.repr max)) p).
 
+Lemma node_rep_saturate_local r p g g_current:
+  node_rep p g g_current r |-- !! is_pointer_or_null p.
+Proof. unfold node_rep; entailer !. Qed.
+Global Hint Resolve node_rep_saturate_local: saturate_local.
+
+Lemma node_rep_valid_pointer t g g_current p: node_rep p g g_current t |-- valid_pointer p.
+Proof.
+  unfold node_rep.
+  Intros.
+  iIntros "(((((H & ?) & ?) & ?) & ?) & ?)".
+  iPoseProof (field_at_valid_ptr0 with "H") as "H"; try auto; simpl; try lia.
+  iVST. entailer !.
+Qed.
+Global Hint Resolve node_rep_valid_pointer : valid_pointer.
+
+
 (* Spec of findnext function *)
 (* FOUND = 0, NOTFOUND = 1, NULLNEXT = 2 (NULLNEXT = NULL || NEXT ) *)
 Definition findnext_spec :=
@@ -694,26 +721,11 @@ Definition findnext_spec :=
                end)
         LOCAL (temp ret_temp (enums stt))
         SEP (match stt with
-               | F | NF => True
-               | NN => !!(n' ∈ extract_node_pn r)
-             end &&
+               | F | NF => data_at sh (tptr t_struct_node) n_pt n
+               | NN => !!(n' ∈ extract_node_pn r) && data_at sh (tptr t_struct_node) next n
+             end *
                node_rep_R r.1.1.1 r.1.2 r.2 g *
-               field_at sh (t_struct_node) [StructField _t] r.1.1.1 p *
-                data_at sh (tptr t_struct_node) next n).
-
-Lemma mylemma pn b:
-   data_at Ews (nested_field_type t_struct_pn (DOT _n)) pn (field_address t_struct_pn (DOT _n) b) |--
-     data_at Ews (tptr t_struct_node) pn (field_address t_struct_pn (DOT _n) b).
-Proof.
-  iIntros.
-  iAssert(!!(nested_field_type t_struct_pn (DOT _n) = tptr t_struct_node)) as "H".
-  {
-    iPureIntro.
-    simpl.
-    auto.
-  }
-  done.
-Qed.
+               field_at sh (t_struct_node) [StructField _t] r.1.1.1 p).
 
 (* Proving inrange spec *)
 Lemma body_inrange: semax_body Vprog Gprog f_inRange inRange_spec.
@@ -753,7 +765,7 @@ Definition traverse_inv (b: val) (n pnN': val) (sh: share)
                         (inv_names : invariants.invG) (g : gname) AS : environ -> mpred :=
   (EX (pnN p: val) (gN_in: gname) (lockN_in: val),
             PROP ()
-            LOCAL (temp _p pnN'; temp _status (vint 2); temp _pn__2 b; temp _x (vint x);
+            LOCAL (temp _p pnN'; temp _flag (vint 2); temp _pn__2 b; temp _x (vint x);
                    (* temp _value v; *) gvars gv)
             SEP (data_at sh (t_struct_pn) (p, pnN) b;
                  in_tree g gN_in pnN lockN_in; in_tree g g_root pnN' lock;
@@ -776,6 +788,16 @@ Definition traverse_inv_2 (b p: val) (sh : share) (x : Z) (g_root g_in g: gname)
 Definition Gprog : funspecs :=
     ltac:(with_library prog [acquire_spec; release_spec; makelock_spec; findnext_spec; 
                              inRange_spec; traverse_spec ]).
+(*
+Axiom node_rep_R_saturate_local: forall t p g_children g,
+  node_rep_R p t g_children g |-- !! is_pointer_or_null p.
+Global Hint Resolve node_rep_R_saturate_local: saturate_local.
+*)
+
+Axiom node_rep_R_valid_pointer: forall t tp g_children g,
+  node_rep_R tp t g_children g |-- valid_pointer tp.
+
+Global Hint Resolve node_rep_R_valid_pointer : valid_pointer.
 
 (* PROVING traverse spec *)
 Lemma traverse: semax_body Vprog Gprog f_traverse traverse_spec.
@@ -783,23 +805,23 @@ Proof.
   start_function.
   Intros p.
   forward.
+  forward.
   set (AS := atomic_shift _ _ _ _ _ ).
   (* New pt: bool * (val * (share * (gname * node_info))) *)
   forward_loop (traverse_inv b n n Ews x v g_root lock gv inv_names g AS)
     break: (*consider to remove gsh *)
-    (EX (stt: enum) (q : val) (gsh: share) (g_in: gname) (r: node_info),
-     PROP() LOCAL(temp _status (enums stt))
-     SEP((match stt with
-            | F => ((traverse_inv_1 b q Ews x g_root g_in g r) *
-                      (!!(r.1.1.1 = nullval) && seplog.emp))
-            | NF => ((traverse_inv_1 b q Ews x g_root g_in g r) *
-                      (!!(r.1.1.1 = nullval) && seplog.emp))
-            | NN => ((traverse_inv_2 b q Ews x g_root g_in g r) *
-                      (!!( r.1.1.1 <> nullval) && seplog.emp)) end) *
-                       Q (stt, (q, (gsh, g_in))) * mem_mgr gv)).
+    (EX (flag: enum) (q : val) (gsh: share) (g_in: gname) (r: node_info),
+     PROP() LOCAL(temp _flag (enums flag))
+     SEP((match flag with
+            | F => ((traverse_inv_2 b q Ews x g_root g_in g r) *
+                      (!!(r.1.1.1 <> nullval) && seplog.emp))
+            | NF => ((traverse_inv_2 b q Ews x g_root g_in g r) *
+                      (!!(r.1.1.1 <> nullval) && seplog.emp))
+            | NN => ((traverse_inv_1 b q Ews x g_root g_in g r) *
+                      (!!( r.1.1.1 = nullval) && seplog.emp)) end) *
+                       Q (flag, (q, (gsh, (g_in, r)))) * mem_mgr gv)).
   - unfold traverse_inv.
-    Exists n p g_root lock. sep_apply in_tree_duplicate. entailer !.
-    Check No_value_for_temp_variable _status. admit.
+    Exists n p g_root lock. sep_apply in_tree_duplicate. entailer !. 
   - (*go deeply into loop*) (*pre-condition*)
     unfold traverse_inv.
     Intros pn p1 g_in lock_in.
@@ -851,29 +873,72 @@ Proof.
     (* inrange function *)
     forward_call(x, pn, (number2Z r.1.2.1), (number2Z r.1.2.2), Ews, gv).
     Intros succ1.
+    assert_PROP(is_pointer_or_null r.1.1.1). entailer !.
     destruct succ1.
     + forward_if.
       forward.
       forward.
-      entailer. admit.
       (*tp = nullval --- pn->p->t == NULL; break*)
-      forward_if. 
-      entailer. admit.
-      viewshift_SEP 0 (EX y, Q y * (in_tree g g_in pn lock_in) *
-                               (!!(y = (NN, (pn, (lsh, g_in)))) && seplog.emp)).
+      forward_if.
+      (* prove r.1.1.2 = lock_in *)
+      gather_SEP (in_tree g g_in pn r.1.1.2) (in_tree g g_in pn lock_in).
+      assert_PROP (r.1.1.2 = lock_in) as Hlk.
+      { sep_apply in_tree_equiv; entailer !. }
+      Intros.
+      rewrite Hlk.
+      (* push back lock into invariant *)
+      gather_SEP AS (in_tree g g_in pn lock_in) (field_at lsh t_struct_node _ _ pn).
+      viewshift_SEP 0 (AS * (in_tree g g_in pn lock_in)).
       {
-        admit.
+        go_lower.
+        iIntros "((AU & #H) & H1)".
+        iMod "AU" as (m) "[Hm HClose]".
+        iPoseProof (in_tree_inv g g_in g_root with "[$H $Hm]") as "InvLock".
+        iDestruct "InvLock" as "(_ & InvLock)".
+        iDestruct "InvLock" as (R) "[H1' H2']".
+        unfold ltree.
+        iDestruct "H1'" as (lsh1) "(%H12 & (H12 & H13))".
+        iAssert(EX lsh0 : share,
+           !! (field_compatible t_struct_node [] pn ∧ readable_share lsh0 ) &&
+           (@field_at CompSpecs lsh0 t_struct_node (DOT _lock) lock_in pn *
+               inv_for_lock lock_in R))
+               with "[H1 H12 H13]" as "H1'".
+        {
+          destruct H12 as (Hf & Hrs).
+          iPoseProof (lock_join with "[H1 H12]") as "H1".
+          { iSplitL "H1"; iFrame; iPureIntro; auto. }
+          iDestruct "H1" as (Lsh) "(% & H1)".
+          iExists _. iFrame; iPureIntro; repeat (split; auto).
+        }
+        iSpecialize ("H2'" with "H1'").
+        iDestruct "HClose" as "(HClose & _)".
+        iSpecialize ("HClose" with "H2'").
+        iMod "HClose". by iFrame.
       }
+      viewshift_SEP 0 (EX y, Q y * (in_tree g g_in pn lock_in) *
+                               (!!(y = (NN, (pn, (Ews, (g_in, r))))) && seplog.emp)).
+      {
+        go_lower.
+        iIntros "(AU & #HITlkin)".
+        iMod "AU" as (m) "[Hm HClose]".
+        iDestruct "HClose" as "[_ HClose]".
+        iSpecialize ("HClose" $! (NN, (pn, (Ews, (g_in, r))))).
+        iFrame "HITlkin".
+        iMod ("HClose" with "[Hm]") as "Hm".
+        iFrame "Hm".
+        iModIntro. iExists _.
+        by iFrame "Hm".
+      }
+      (*proving it satisfies with the post condition of traverse *)
+      Intros y.
       forward.
-      simpl.
-      Exists  (NN, (pn, (lsh, g_in))). entailer !. admit.
+      Exists NN pn Ews g_in r.
+      unfold traverse_inv_1.
+      unfold node_lock_inv_pred, node_rep.
+      entailer !.
+      by iIntros "_".
       forward.
-      Check StructField _n.
-      Check field_address.
-      Check field_at.
-      Check field_address _ [StructField _n] _.
       assert_PROP(field_compatible t_struct_pn (DOT _n) b). entailer !.
-      (* x: Z, p: val, n: val, n_pt: val, r: node_info, g: gname, sh: share, gv: globals *)
       (* findNext *)
       forward_call(x, pn, (field_address t_struct_pn [StructField _n] b),
                    pn, r, g, Ews, gv).
@@ -885,7 +950,7 @@ Proof.
         Intros succ.
         (* assert_PROP(r.1.1.1 <> nullval) by entailer !. *)
         destruct succ.1.1; last first.
-        Intros.
+        Intros. 
         * (* NN => succ.1.2 = succ.2  *)
           (* not found and find the next point *)
           forward.
@@ -924,11 +989,12 @@ Proof.
             { rewrite <- Hlk. iFrame "H". done. }
             iExists g_in1, lock1.
             iSpecialize ("HClose" with "H1").
-            rewrite H9.
+            rewrite H11.
             by iFrame "Inv H2".
           }
           (*Now we have in_tree g succ.2 pnext lknext *)
           Intros gnext lknext.
+          Search is_pointer_or_null.
           (* _release(_t'8);) *)
           forward_call release_inv (lock_in, node_lock_inv_pred g pn g_in r, AS).
           {
@@ -936,7 +1002,7 @@ Proof.
             iIntros "(((((((HAS & H1) & H2) & H3) & H4) & H5) & H6) & H7)".
             iCombine "HAS H1 H3 H2 H4 H5 H6 H7" as "Hnode_inv_pred".
             iVST.
-            rewrite <- H9.
+            rewrite <- H11.
             rewrite <- 2sepcon_assoc; rewrite <- 2sepcon_comm.
             apply sepcon_derives; [| cancel_frame].
             unfold atomic_shift;
@@ -972,59 +1038,166 @@ Proof.
          entailer !. admit.
          unfold_data_at (data_at Ews t_struct_pn _ b).
          cancel.
-       * rewrite TT_andp.
+       * (* NF case *)
          forward.
          forward_if.
          forward.
          easy.
          forward_if.
-         forward.
-         (*
-           EX a : enum * (val * (share * gname)), !! (vint 1 = enums a.1) && (Q a * mem_mgr gv)
-          *)
-         admit.
-
-         forward.
-         forward.
-         easy.
-       * rewrite TT_andp.
-         forward.
-         forward_if.
-         forward.
-         admit.
-         (* contradiction *)
-         easy.
-     }
-     (* contradiction *)
-     easy.
-    + forward_if.
+         gather_SEP (in_tree g g_in pn r.1.1.2) (in_tree g g_in pn lock_in).
+         assert_PROP (r.1.1.2 = lock_in) as Hlk.
+         { sep_apply in_tree_equiv; entailer !. }
+         Intros.
+         rewrite Hlk.
+         (* push back lock into invariant *)
+         gather_SEP AS (in_tree g g_in pn lock_in) (field_at lsh t_struct_node _ _ pn).
+         viewshift_SEP 0 (AS * (in_tree g g_in pn lock_in)).
+         {
+           go_lower.
+           iIntros "((AU & #H) & H1)".
+           iMod "AU" as (m) "[Hm HClose]".
+           iPoseProof (in_tree_inv g g_in g_root with "[$H $Hm]") as "InvLock".
+           iDestruct "InvLock" as "(_ & InvLock)".
+           iDestruct "InvLock" as (R) "[H1' H2']".
+           unfold ltree.
+           iDestruct "H1'" as (lsh1) "(%K12 & (H12 & H13))".
+           iAssert(EX lsh0 : share,
+                      !! (field_compatible t_struct_node [] pn ∧ readable_share lsh0 ) &&
+                        (@field_at CompSpecs lsh0 t_struct_node (DOT _lock) lock_in pn *
+               inv_for_lock lock_in R))
+               with "[H1 H12 H13]" as "H1'".
+        {
+          destruct K12 as (Hf & Hrs).
+          iPoseProof (lock_join with "[H1 H12]") as "H1".
+          { iSplitL "H1"; iFrame; iPureIntro; auto. }
+          iDestruct "H1" as (Lsh) "(% & H1)".
+          iExists _. iFrame; iPureIntro; repeat (split; auto).
+        }
+        iSpecialize ("H2'" with "H1'").
+        iDestruct "HClose" as "(HClose & _)".
+        iSpecialize ("HClose" with "H2'").
+        iMod "HClose". by iFrame.
+      }
+      viewshift_SEP 0 (EX y, Q y * (in_tree g g_in pn lock_in) *
+                               (!!(y = (NF, (succ.1.2, (Ews, (g_in, r))))) && seplog.emp)).
+      {
+        go_lower.
+        iIntros "(AU & #HITlkin)".
+        iMod "AU" as (m) "[Hm HClose]".
+        iDestruct "HClose" as "[_ HClose]".
+        iSpecialize ("HClose" $! (NF, (succ.1.2, (Ews, (g_in, r))))).
+        iFrame "HITlkin".
+        iMod ("HClose" with "[Hm]") as "Hm".
+        iFrame "Hm".
+        iModIntro. iExists _.
+        by iFrame "Hm".
+      }
+      Intros y.
+      rewrite <- H11.
+      forward.
+      Exists  (NF, (succ.1.2 , (Ews, (g_in, r)))).
+      simpl.
+      unfold node_lock_inv_pred, node_rep.
+      simpl.
+      entailer !.
+      unfold_data_at (data_at Ews t_struct_pn _ b).
+      cancel.
+      by iIntros "_".
+      (* contradiction *)
       easy.
-      forward.
-      forward.
+    * forward.
+      forward_if.
       gather_SEP (in_tree g g_in pn r.1.1.2) (in_tree g g_in pn lock_in).
       assert_PROP (r.1.1.2 = lock_in) as Hlk.
       { sep_apply in_tree_equiv; entailer !. }
-      rewrite Hlk.
       Intros.
+      rewrite Hlk.
       (* push back lock into invariant *)
       gather_SEP AS (in_tree g g_in pn lock_in) (field_at lsh t_struct_node _ _ pn).
       viewshift_SEP 0 (AS * (in_tree g g_in pn lock_in)).
-      { go_lower; apply push_lock_back; auto. }
-      Intros.
-      gather_SEP AS (in_tree g g_in pn lock_in) (node_rep_R r.1.1.1 r.1.2 r.2 g)
+      {
+        go_lower.
+        iIntros "((AU & #H) & H1)".
+        iMod "AU" as (m) "[Hm HClose]".
+        iPoseProof (in_tree_inv g g_in g_root with "[$H $Hm]") as "InvLock".
+        iDestruct "InvLock" as "(_ & InvLock)".
+        iDestruct "InvLock" as (R) "[H1' H2']".
+        unfold ltree.
+        iDestruct "H1'" as (lsh1) "(%K12 & (H12 & H13))".
+        iAssert(EX lsh0 : share,
+                      !! (field_compatible t_struct_node [] pn ∧ readable_share lsh0 ) &&
+                        (@field_at CompSpecs lsh0 t_struct_node (DOT _lock) lock_in pn *
+               inv_for_lock lock_in R))
+               with "[H1 H12 H13]" as "H1'".
+        {
+          destruct K12 as (Hf & Hrs).
+          iPoseProof (lock_join with "[H1 H12]") as "H1".
+          { iSplitL "H1"; iFrame; iPureIntro; auto. }
+          iDestruct "H1" as (Lsh) "(% & H1)".
+          iExists _. iFrame; iPureIntro; repeat (split; auto).
+        }
+        iSpecialize ("H2'" with "H1'").
+        iDestruct "HClose" as "(HClose & _)".
+        iSpecialize ("HClose" with "H2'").
+        iMod "HClose". by iFrame.
+      }
+      viewshift_SEP 0 (EX y, Q y * (in_tree g g_in pn lock_in) *
+                               (!!(y = (F, (succ.1.2, (Ews, (g_in, r))))) && seplog.emp)).
+      {
+        go_lower.
+        iIntros "(AU & #HITlkin)".
+        iMod "AU" as (m) "[Hm HClose]".
+        iDestruct "HClose" as "[_ HClose]".
+        iSpecialize ("HClose" $! (F, (succ.1.2, (Ews, (g_in, r))))).
+        iFrame "HITlkin".
+        iMod ("HClose" with "[Hm]") as "Hm".
+        iFrame "Hm".
+        iModIntro. iExists _.
+        by iFrame "Hm".
+      }
+      Intros y.
+      rewrite <- H11.
+      forward.
+      Exists  (F, (succ.1.2 , (Ews, (g_in, r)))).
+      simpl.
+      unfold node_lock_inv_pred, node_rep.
+      simpl.
+      entailer !.
+      unfold_data_at (data_at Ews t_struct_pn _ b).
+      cancel.
+      by iIntros "_".
+      (* contradiction *)
+      easy.
+    }
+    easy.
+  + forward_if.
+    easy.
+    forward.
+    forward.
+    gather_SEP (in_tree g g_in pn r.1.1.2) (in_tree g g_in pn lock_in).
+    assert_PROP (r.1.1.2 = lock_in) as Hlk.
+    { sep_apply in_tree_equiv; entailer !. }
+    rewrite Hlk.
+    Intros.
+      (* push back lock into invariant *)
+    gather_SEP AS (in_tree g g_in pn lock_in) (field_at lsh t_struct_node _ _ pn).
+    viewshift_SEP 0 (AS * (in_tree g g_in pn lock_in)).
+    { go_lower; apply push_lock_back; auto. }
+    Intros.
+    gather_SEP AS (in_tree g g_in pn lock_in) (node_rep_R r.1.1.1 r.1.2 r.2 g)
                         (field_at _ _ _ _ pn)
                         (field_at Ews t_struct_node _ _ pn)
                         (field_at Ews t_struct_node _ _ pn)
                         (malloc_token Ews t_struct_node pn) (my_half g_in Tsh r).
-      viewshift_SEP 0 (AS * (node_lock_inv_pred g pn g_in r )).
-      {
+    viewshift_SEP 0 (AS * (node_lock_inv_pred g pn g_in r )).
+    {
             go_lower.
             iIntros "(((((((AU & #H) & HNode) & H2) & H3) & H4) & H5) & H6)".
             iFrame.
             rewrite <- Hlk. iFrame "H". done.
-      }
-      forward_call release_inv (lock_in, node_lock_inv_pred g pn g_in r, AS).
-      {
+    }
+    forward_call release_inv (lock_in, node_lock_inv_pred g pn g_in r, AS).
+    {
         lock_props.
         iIntros "(((((HAS & H1) & H2) & H3) & H4) & H5)".
         iCombine "HAS H1 H2 H3 H4 H5" as "Hnode_inv_pred".
@@ -1056,19 +1229,23 @@ Proof.
           iSpecialize ("HI2" with "H").
           iDestruct "HClose" as "[HClose _]". 
           by iSpecialize ("HClose" with "HI2").
-       }
-       (* proving |--  traverse_inv *)
+     }
+     (* proving |--  traverse_inv *)
        forward.
        unfold traverse_inv.
        Exists n pn g_root lock.
        sep_apply (in_tree_duplicate g g_root n).
        entailer !.
+   
+       
     - (* semax Delta (PROP ( )  RETURN ( ) SEP ()) (return _flag;) POSTCONDITION *)
        Intros flag.
        Intros pn gsh g_in r.
        unfold traverse_inv_1, traverse_inv_2.
        destruct flag.
-       + forward.
+       + simpl.
+         autorewrite with norm.
+         forward.
          Exists (true, (pn, (gsh, (g_in, r)))).
          simpl. entailer !. 
        + forward.
